## Waves on rectangular domain

You find content related to this lecture in the textbooks:

- @baldock section 7.4
- @coulson section 33

<iframe src="https://york.cloud.panopto.eu/Panopto/Pages/Embed.aspx?id=8a76711e-1f8b-4afd-bbb3-af790124753e&autoplay=false&offerviewer=true&showtitle=true&showbrand=false&captions=true&interactivity=all" height="405" width="720" style="border: 1px solid #464646;" allowfullscreen allow="autoplay"></iframe>

Consider a rectangular membrane: $D=\{(x,y)\in\mathbb{R}^2\vert 0<x<a, \ 0<y<b \}$. 
Let's solve the wave equation
$$
\partial_t^2 \, z -c^2 \, \left(\partial_x^2 \, z + \partial_y^2 \, z\right)=0 \quad \text{in} \ \ D
$$ {#eq-rectangular1}
subject to the fixed (Dirichlet) boundary condition
$$
z(x,y,t)=0 \quad \text{on} \ \ \partial D
$$ {#eq-rectangular2}
or, equivalently,
$$
z(0,y,t)=0, \quad z(a,y,t)=0
$$ {#eq-rectangular3}
and
$$
z(x,0,t)=0, \quad z(x,b,t)=0.
$$ {#eq-rectangular4}
To find a solution, we use the method of separation of variables (see 
@sec-4.1), i.e., we make the Ansatz
$$
z(x,y,t)=X(x)Y(y)T(t).
$$ {#eq-8.5}
Substituting this Ansatz into the wave equation, we get
$$
XYT''=c^2\left(X''YT + XY''T\right),
$$ {#eq-8.6}
which, after dividing by $XYT$ gives
$$
\frac{T''(t)}{T(t)} = c^2\left(\frac{X''(x)}{X(x)}
+\frac{Y''(y)}{Y(y)}\right).
$$ {#eq-8.7}
In the last equation, we have a function of one variable, $t$, on the left side
and a function of two different variables, $x$ and $y$, on the right side. The equation can be
satisfied for all $x$, $y$ and $t$ only if both sides are equal to a constant.
As in @sec-4.1, we choose this constant to be negative and (for
convenience) equal to $-k^2 c^2$ (for arbitrary real $k$). Again, the
possibility of a positive constant is excluded, because with a positive
constant it is impossible to find solutions satisfying the boundary conditions.
Thus, we have
$$
\frac{T''(t)}{T(t)} = c^2\left(\frac{X''(x)}{X(x)}
+\frac{Y''(y)}{Y(y)}\right)= -k^2 c^2.
$$ {#eq-8.8}
This leads to the ODE
$$
T''(t)=-c^2 k^2  \, T(t)
$$ {#eq-rectangular5}
and to the equation
$$
\frac{X''(x)}{X(x)}
+\frac{Y''(y)}{Y(y)}= -k^2.
$$ {#eq-rectangular6}
The general solution of @eq-rectangular5 is
$$
T(t)=F \, \sin(k c t) +G \, \cos(k c t),
$$ {#eq-rectangular7}
where $F$ and $G$ are arbitrary constants.

Rewriting @eq-rectangular6 as
$$
\frac{X''(x)}{X(x)}= -k^2 -\frac{Y''(y)}{Y(y)},
$$ {#eq-8.12}
we conclude that for this equation to hold for all $x$ and $y$, both sides must
be equal to a constant, which we choose to write as $-\nu^2$ (for some real $\nu$).
Also, introducing the constant $\mu$ so that $\nu^2+\mu^2=k^2$ gives us the equations
$$
X''(x) =-\nu^2 X(x), \quad Y''(y)=-\mu^2Y(y).
$$ {#eq-rectangular8}

The general solutions are
$$\begin{split}
X(x)&=A\sin(\nu x)+ B\cos(\nu x),\\
Y(y)&=C\sin(\mu y)+ D\cos(\mu y),
\end{split}$$ {#eq-8.14}
for arbitrary constants $A,B,C,D$. 

Now we are ready to impose the boundary conditions. 

The condition
$z(0,y,t)=0$ for all $y,t$ requires that $X(0)=0$ and, because $X(0)= B$, this
implies that $B=0$. Similarly the condition $z(a,y,t)=0$ requires that $X(a)=0$
and because $X(a)=A\sin(\nu\, a)$ (because we already know that $B=0$), this
implies that either $A=0$, which is not an interesting case because it makes the
entire solution vanish, or that $\nu=n\pi/a$ with $n\in \mathbb{Z}$. Without loss of
generality we can take $n\in\mathbb{N}$ because negative $n$ just give the same
solution up to a sign that can be absorbed into the arbitrary constant $A$, and
$n=0$ gives the zero solution.

The conditions $z(x,0,t)=0=z(x,b,t)$ similarly require that $Y(0)=0=Y(\pi)$
and thus $D=0$ and $\mu=m\pi/a$ with $m\in\mathbb{N}$.

Thus we have found the following solutions satisfying the boundary conditions:
$$\begin{split}
z_{nm}(x,y,t)=&\sin\left(\frac{\pi}{a}nx\right)\sin\left(\frac{\pi}{b}my\right)\\
&\cdot\left(F_{nm}\sin(k_{nm}ct)+G_{nm}\cos(k_{nm}ct)\right)
\end{split}$${#eq-rectangular12}
with 
$$
k_{nm}=\sqrt{\left(\frac{n\pi}{a}\right)^2+\left(\frac{m\pi}{b}\right)^2}
$$ {#eq-8.16}
for any choice of $n,m\in\mathbb{N}$ and $F_{nm},G_{nm}\in\mathbb{R}$.

Note that solutions @eq-rectangular12 already satisfy the boundary conditions
@eq-rectangular3 and @eq-rectangular4. Such solutions are called _normal modes_
of the membrane. Snapshots of normal modes with $(n,m)=(1,1)$, $(n,m)=(1,2)$,
$(n,m)=(2,2)$ and $(n,m)=(3,2)$ are shown in @fig-rectangular_membrane. 

![Some normal modes of a rectangular membrane](rectangular_membrane){#fig-rectangular_membrane}

The amplitudes of the normal modes oscillate over time. The following video shows an animation of various normal modes:
{{< video https://youtu.be/yDZsCZn3lSk >}}

Any
solution of the wave equation @eq-rectangular1 satisfying the boundary
conditions @eq-rectangular3 and @eq-rectangular4 can be presented as a linear
combination of normal modes @eq-rectangular12:

$$
z(x,y,t)=\sum_{n=1}^\infty\sum_{m=1}^\infty z_{nm}.
$$ {#eq-8.17}
The free constants $F_{nm}$ and $G_{nm}$ are then determined by the initial
conditions, using the Fourier transform technique as in the one-dimensional
case.


To construct a solution satisfying the initial conditions
$$
z(x,y,0)=z_0(x,y), \quad \partial_t z(x,y,0)=v_0(x,y)
$$ {#eq-8.18}
we evaluate our general solution and its $t$ derivative at the boundary. This gives
$$
z(x,y,0)=\sum_{n=1}^{\infty}\sum_{m=1}^{\infty} 
\sin\frac{\pi n x}{a} \, \sin\frac{\pi m y}{b} G_{nm}= z_0(x,y),
$$ {#eq-8.19}
$$
\partial_t z(x,y,0)=\sum_{n=1}^{\infty}\sum_{m=1}^{\infty} k_{nm} c \,
B_{nm} \, \sin\frac{\pi n x}{a} \, \sin\frac{\pi m y}{b}=v_0(x,y).
$$ {#eq-8.20}
Comparing these with the (double) Fourier series for functions $z_0(x,y)$ and $v_0(x,y)$, one can deduce that
$$\begin{split}
G_{nm} &= \frac{4}{ab} \, \int\limits_{0}^{a} dx \int\limits_{0}^{b}  dy \,  z_0(x,y)
\sin\frac{\pi n x}{a} \, \sin\frac{\pi m y}{b},  \\
F_{nm} &= \frac{1}{k_{nm}c} \, \frac{4}{ab} \, \int\limits_{0}^{a} dx \int\limits_{0}^{b}  dy \, v_0(x,y)
\sin\frac{\pi n x}{a} \, \sin\frac{\pi m y}{b}.  
\end{split}$$ {#eq-8.21}
