# Bernoulli's solution

You find content related to this lecture in the textbooks:

- @knobel sections 11.2 and 11.3, chapters 13 and 14
- @baldock sections 3.1, 3.2, 3.3
- @simmons sections 39 and 40

We will now solve the wave equation again in a totally different way from
d'Alembert, following instead Bernoulli. This is a method you have seen before,
namely the method of separation of variables.

## Separation of variables {#sec-4.1}
We make the Ansatz that the solution factorises into one function of only $x$
and one function of only $t$:
$$
y(x,t) = X(x)T(t).
$$ {#eq-4.1}
Substituting this into the wave equation
$$
\partial_x^2y(x,t)=\frac{1}{c^2}\partial_t^2y(x,t)
$$ {#eq-4.2}
 we get
$$
X''(x)T(t)=\frac{1}{c^2}X(x)T''(t) .
$$ {#eq-4.3}
We divide both sides by $X(x)T(t)$, which will separate the variables:
$$
\frac{X''(x)}{X(x)}=\frac{1}{c^2}\frac{T''(t)}{T(t)}.
$$ {#eq-4.4}
It the last equation, we have a function of $x$ only on the left hand side and a
function of $t$ only on the right hand side. The equation must hold for all $x$
and $t$. This is only possible if both functions are equal to a constant. It
will turn out to be convenient to write this constant as $-k^2$ for some new
constant $k$. Thus we set
$$
\frac{X''(x)}{X(x)}=\frac{1}{c^2}\frac{T''(t)}{T(t)} =- k^2.
$$ {#eq-4.5}
This means that $X(x)$ and $T(t)$ must be solutions of the ODEs
$$
X''=-k^2 X \quad \text{and}\quad T''=-k^2 c^2 T.
$$ {#eq-4.6}
The general solutions of these ODEs are
$$\begin{split}
X(x)&= A \, \sin(kx) + B \, \cos(kx), \\
T(t)&= F \, \sin(kct) + G \, \cos(kct),
\end{split}$$ {#eq-4.7}
where $A, B, F, G$ and $k$ are arbitrary constants.

## Finite string with fixed ends

Bernoulli was most interested in the finite string. Let us put the ends of the
string at $x=0$ and $x=\pi$. Now let the ends of the string be fixed. This means
that we need to impose homogeneous Dirichlet boundary conditions
$$
y(0,t)=0 \quad \text{and} \quad y(\pi,t)=0 \quad \text{for all} \ \ t .
$$ {#eq-finitestr2}
These conditions will be satisfied if $X(0)=0$ and $X(\pi)=0$. Imposing the
condition $X(0)=0$ on the general solution for $X(x)$, we find that we need
$B=0$. We then have from $X(\pi)=0$ that
$$
A\sin(k\pi) = 0.
$$ {#eq-4.9}
The last equation implies that either $A=0$ or $\sin(k\pi)=0$. We reject the
first option because it results in a zero solution. The second option yields
$$
\sin(k\pi) = 0 \quad \Rightarrow k\in\mathbb{Z}.
$$ {#eq-4.10}

Thus, for each positive integer $k$ we have a solution of the wave equation of
the form
$$
y_k(x,t) = \sin\left(k x\right)\left(F_k \, \sin(k c t) + G_k \, \cos(k c t)\right)
$$ {#eq-finitestr3}
^[We do not need negative $k$ because they will produce the same solutions, and
we do not need $k=0$ because it yields zero solution. Also, we have absorbed the
constant $A$ into the constants $F_k$ and $G_k$.]

## Standing waves

The solutions we obtained in the previous section are standing waves. They don't
change their shape and don't move, only their amplitude oscillates with time. In
the lecture videos I make various sketches and animations to illustrate this.

So we now have a stark contrast between what d'Alembert found and what Bernoulli
found. According to d'Alembert, the solutions of the wave equation are
travelling waves of arbitrary shape. According to Bernoulli, the solutions are
standing waves that have sine shape. It is always wonderful when one has two
very different ways of looking at the same phenomenon. That is where deep
understanding comes from.

The resolution of the apparent paradox is that a superposition of standing waves
can give a travelling wave, and that a superposition of sine waves can give any
shape.

## Initial value problem

Since the wave equation is linear and also the boundary conditions we imposed
were linear, a linear combination of any number of the solutions is also a
solution (this is called the _superposition principle_. So, we can construct a
general solution of the wave equation by summing up the harmonic standing waves
from @eq-finitestr3:
$$
y(x,t) = \sum_{k=1}^{\infty}\sin\left(k x\right)\left(F_k \, \sin(k c t) + G_k \, \cos(k c t)\right). 
$$ {#eq-finitestr4}
Here the $G_k$ and the $F_k$ are undetermined constants, to be fixed from the
initial conditions.

Suppose now that we are given the initial conditions
$$
y(x,0) = y_0(x), \quad \pr_t y(x,0)=v_0(x) \quad \text{for } x\in[0,\pi].
$$ {#eq-finitestr5}
How to choose constants $F_k$ and $G_k$ so as to satisfy the initial conditions?
Let's substitute @eq-finitestr4 into @eq-finitestr5. We have
$$
y_0(x) = \sum_{k=1}^{\infty}G_k \, \sin\left(k x\right), \quad
v_0(x) = \sum_{k=1}^{\infty}F_k\, k c \, \sin\left(k x\right).
$$ {#eq-finitestr6}
These formulae look like Fourier series for the functions $y_0$ and $v_0$. So,
to find coefficients $F_k$ and $G_k$, we use the identity
$$
\int\limits_{0}^{\pi}\sin\left(k x\right)\sin(l x)dx = \frac{\pi}{2}\delta_{kl},
$$
where $\delta_{kl}$ is the Kronecker delta:
$$
 \delta_{kl} =\begin{cases}
1 &\text{if \ } k=l \\
0 &\text{if \ } k\neq l
\end{cases}
$$
To make use of this, we multiply each of @eq-finitestr6 by $2/\pi \,\sin(l x)$
and integrate over the interval $[0,\pi]$:
$$\begin{split}
\frac{2}{\pi}\int\limits_{0}^{\pi}y_0(x)\sin(l x)dx 
&=\frac{2}{\pi} \sum_{k=1}^{\infty}G_k \, \int\limits_{0}^{\pi}\sin\left(k x\right)\sin(l x)dx\\
&=\sum_{k=1}^{\infty}G_k \delta_{kl}=G_l
\end{split}
$$ {#eq-finitestr7}
$$\begin{split}
\frac{2}{\pi}\int\limits_{0}^{\pi}v_0(x)\sin(l x)dx &= 
\frac{2}{\pi}\sum_{k=1}^{\infty}F_k\, k c \, \int\limits_{0}^{\pi}\sin\left(k x\right)\sin(l x)dx\\
&=\sum_{k=1}^{\infty}F_k\, k c\, \delta_{kl}= F_l\, l c
\end{split}
$$ {#eq-finitestr8}
Thus we know how to determine the constants $F_k$ and $G_k$ in the general
solution @eq-finitestr4 such as to satisfy given initial conditions.
